Made some name changes to normalize the TraceInclusions file.

Properties.v
@@ -1838,7 +1838,7 @@ Section StepSimulation.
           rewrite nthProp2_cons; split; auto.
   Qed.
 
-  Theorem StepSimulation:
+  Theorem _StepSimulation:
     TraceInclusion imp spec.
   Proof.
     unfold TraceInclusion; intros.
@@ -1889,10 +1889,10 @@ Section SimulationZero.
              UpdRegs [uSpec] oSpec oSpec' /\
              simRel oImp' oSpec')).
 
-  Theorem simulationZero:
+  Theorem _simulationZero:
     TraceInclusion (Base imp) (Base spec).
   Proof.
-    apply StepSimulation with (simRel := simRel); auto; intros.
+    apply _StepSimulation with (simRel := simRel); auto; intros.
     inv H.
     pose proof HSubsteps as sth.
     inv HSubsteps; simpl in *.
@@ -3522,7 +3522,7 @@ Proof.
   split; induction 1; econstructor; eauto.
 Qed.
 
-Theorem flatten_WfMod m: WfMod m -> WfMod (flatten m).
+Theorem _flatten_WfMod m: WfMod m -> WfMod (flatten m).
 Proof.
   unfold flatten.
   induction 1; simpl; auto; intros.
@@ -3569,7 +3569,7 @@ Proof.
 Qed.
 
 Definition flattened_ModWf m: ModWf :=
-  (Build_ModWf (flatten_WfMod (wfMod m))).
+  (Build_ModWf (_flatten_WfMod (wfMod m))).
 
 Section TraceSubstitute.
   Variable m: ModWf.
@@ -3600,7 +3600,7 @@ Section TraceSubstitute.
       + destruct m; auto.
   Qed.
 
-  Theorem TraceInclusion_flatten_r: TraceInclusion m (flattened_ModWf m).
+  Theorem _TraceInclusion_flatten_r: TraceInclusion m (flattened_ModWf m).
   Proof.
     unfold TraceInclusion; intros.
     exists o1, ls1.
@@ -3608,7 +3608,7 @@ Section TraceSubstitute.
     apply Trace_flatten_same1; auto.
   Qed.
 
-  Theorem TraceInclusion_flatten_l: TraceInclusion (flattened_ModWf m) m.
+  Theorem _TraceInclusion_flatten_l: TraceInclusion (flattened_ModWf m) m.
   Proof.
     apply TraceInclusion'_TraceInclusion.
     unfold TraceInclusion'; intros.
@@ -3860,7 +3860,7 @@ Section ModularSubstitution.
   Variable wfAConcatB: WfMod (ConcatMod a b).
   Variable wfA'ConcatB': WfMod (ConcatMod a' b').
 
-  Theorem ModularSubstitution: TraceInclusion a a' ->
+  Theorem _ModularSubstitution: TraceInclusion a a' ->
                              TraceInclusion b b' ->
                              TraceInclusion (ConcatMod a b) (ConcatMod a' b').
   Proof.
@@ -4150,7 +4150,7 @@ Section SimulationZeroAct.
                  UpdRegs [uSpec] oSpec oSpec' /\
                  simRel oImp' oSpec')).
 
-  Theorem simulationZeroAct:
+  Theorem _simulationZeroAct:
     TraceInclusion (Base imp) (Base spec).
   Proof.
     pose proof (wfBaseModule imp) as wfImp.
@@ -4158,7 +4158,7 @@ Section SimulationZeroAct.
     inv wfImp.
     inv wfSpec.
     dest.
-    apply simulationZero with (simRel := simRel); auto; simpl; intros.
+    apply _simulationZero with (simRel := simRel); auto; simpl; intros.
     inv H9; [|discriminate].
     inv HLabel.
     specialize (@simulation oImp reads u rn cs oImp' rb HInRules HAction H10 _ H11).
@@ -4358,7 +4358,7 @@ Section SimulationGen.
         tauto.
   Qed.
         
-  Theorem simulationGen:
+  Theorem _simulationGen:
     TraceInclusion (Base imp) (Base spec).
   Proof.
     pose proof (wfBaseModule imp) as wfImp.
@@ -4366,7 +4366,7 @@ Section SimulationGen.
     inv wfImp.
     inv wfSpec.
     dest.
-    apply StepSimulation with (simRel := simRel); auto; simpl; intros.
+    apply _StepSimulation with (simRel := simRel); auto; simpl; intros.
     inv H9.
     pose proof (SubstepsSingle HSubsteps) as sth.
     destruct lImp; [tauto| simpl in *].
@@ -4828,10 +4828,10 @@ Section SimulationGeneralEx.
       SemAction oImp (aImp2 type arg2) rImpl2 uImpl2 csImp2 ret2 ->
       exists k, In k (map fst uImpl1) /\ In k (map fst uImpl2).
 
-  Theorem simulationGeneralEx:
+  Theorem _simulationGeneralEx:
     TraceInclusion (Base imp) (Base spec).
   Proof.
-    eapply simulationGen; eauto; intros.
+    eapply _simulationGen; eauto; intros.
     - pose proof (SemAction_NoDup_u H0) as sth.
       pose proof (simRelImpGood H2) as sth2.
       apply (f_equal (map fst)) in sth2.
@@ -4888,10 +4888,10 @@ Section SimulationZeroA.
                  UpdRegs [uSpec] oSpec oSpec' /\
                  simRel (doUpdRegs uImp oImp) oSpec')).
 
-  Theorem simulationZeroA:
+  Theorem _simulationZeroA:
     TraceInclusion (Base imp) (Base spec).
   Proof.
-    eapply simulationZeroAct; eauto; intros.
+    eapply _simulationZeroAct; eauto; intros.
     pose proof (SemAction_NoDup_u H0) as sth.
     pose proof (simRelImpGood H2) as sth2.
     apply (f_equal (map fst)) in sth2.
@@ -4959,10 +4959,10 @@ Section SimulationGeneral.
       SemAction oImp (aImp2 type arg2) rImpl2 uImpl2 csImp2 ret2 ->
       exists k, In k (map fst uImpl1) /\ In k (map fst uImpl2).
 
-  Theorem simulationGeneral:
+  Theorem _simulationGeneral:
     TraceInclusion (Base imp) (Base spec).
   Proof.
-    eapply simulationGeneralEx; eauto; intros.
+    eapply _simulationGeneralEx; eauto; intros.
     - specialize (@simulationRule _ _ _ _ _ _ H H0 oSpec H1).
       destruct simulationRule; auto.
       dest.
@@ -5030,10 +5030,10 @@ Section SimulationZeroAction.
                SemAction oSpec (aSpec type) rSpec uSpec csImp WO /\
                  simRel (doUpdRegs uImp oImp) (doUpdRegs uSpec oSpec))).
 
-  Theorem simulationZeroAction:
+  Theorem _simulationZeroAction:
     TraceInclusion (Base imp) (Base spec).
   Proof.
-    eapply simulationZeroA; eauto; intros.
+    eapply _simulationZeroA; eauto; intros.
     specialize (@simulation _ _ _ _ _ _ H H0 _ H1).
     destruct simulation; auto.
     right.
@@ -5093,7 +5093,7 @@ Ltac discharge_NoSelfCall :=
          end.
 
 Ltac discharge_simulationGeneral mySimRel disjReg :=
-  apply simulationGeneral with (simRel := mySimRel); auto; simpl; intros;
+  apply _simulationGeneral with (simRel := mySimRel); auto; simpl; intros;
   (repeat match goal with
           | H: _ \/ _ |- _ => destruct H
           | H: False |- _ => exfalso; apply H
