TraceInclusions.v
@@ -4,7 +4,7 @@ Require Import Kami.Properties.
 Require Import Kami.PProperties.
 Require Import Kami.PPlusProperties.
 
-Theorem _StepSimulation (imp spec : Mod) (simRel : RegsT -> RegsT -> Prop)
+Theorem StepSimulation (imp spec : Mod) (simRel : RegsT -> RegsT -> Prop)
         (initRel : forall rimp : list RegT,
             Forall2 regInit rimp (getAllRegisters imp)
             -> exists rspec, Forall2 regInit rspec (getAllRegisters spec)
@@ -22,10 +22,10 @@ Theorem _StepSimulation (imp spec : Mod) (simRel : RegsT -> RegsT -> Prop)
                 simRel oImp' oSpec' /\ WeakInclusion lImp lSpec) :
   TraceInclusion imp spec.
 Proof.
-  eauto using StepSimulation.
+  eauto using _StepSimulation.
 Qed.
 
-Theorem _simulationZero (imp spec : BaseModule) (simRel : RegsT -> RegsT -> Prop)
+Theorem simulationZero (imp spec : BaseModule) (simRel : RegsT -> RegsT -> Prop)
         (initRel : forall rimp : list RegT,
             Forall2 regInit rimp (getAllRegisters imp)
             -> exists rspec, Forall2 regInit rspec (getAllRegisters spec)
@@ -46,28 +46,30 @@ Theorem _simulationZero (imp spec : BaseModule) (simRel : RegsT -> RegsT -> Prop
                   simRel oImp' oSpec') :
   TraceInclusion (Base imp) (Base spec).
 Proof.
-  eauto using simulationZero.
+  eauto using _simulationZero.
 Qed.
 
-Theorem _flatten_WfMod m :
+Theorem flatten_WfMod m :
   WfMod m -> WfMod (flatten m).
 Proof.
-  eauto using flatten_WfMod.
+  eauto using _flatten_WfMod.
 Qed.
 
-Theorem _TraceInclusion_flatten_r (m : ModWf) :
-  TraceInclusion m (flattened_ModWf m).
+Definition flatten_ModWf m := flattened_ModWf m.
+
+Theorem TraceInclusion_flatten_r (m : ModWf) :
+  TraceInclusion m (flatten_ModWf m).
 Proof.
-  eauto using TraceInclusion_flatten_r.
+  eauto using _TraceInclusion_flatten_r.
 Qed.
 
-Theorem _TraceInclusion_flatten_l (m : ModWf) :
-  TraceInclusion (flattened_ModWf m) m.
+Theorem TraceInclusion_flatten_l (m : ModWf) :
+  TraceInclusion (flatten_ModWf m) m.
 Proof.
-  eauto using TraceInclusion_flatten_l.
+  eauto using _TraceInclusion_flatten_l.
 Qed.
 
-Theorem _ModularSubstitution (a b a' b' : Mod)
+Theorem ModularSubstitution (a b a' b' : Mod)
         (SameList_a : forall x,
             (In x (map fst (getAllMethods a)) /\
              ~ In x (getHidden a)) <->
@@ -84,10 +86,10 @@ Theorem _ModularSubstitution (a b a' b' : Mod)
   TraceInclusion b b' ->
   TraceInclusion (ConcatMod a b) (ConcatMod a' b').
 Proof.
-  eauto using ModularSubstitution.
+  eauto using _ModularSubstitution.
 Qed.
 
-Theorem _simulationZeroAct (imp spec : BaseModuleWf) (simRel : RegsT -> RegsT -> Prop)
+Theorem simulationZeroAct (imp spec : BaseModuleWf) (simRel : RegsT -> RegsT -> Prop)
         (simRelGood : forall oImp oSpec : RegsT,
         simRel oImp oSpec -> getKindAttr oSpec = getKindAttr (getRegisters spec))
         (initRel : forall rimp : list RegT,
@@ -112,10 +114,10 @@ Theorem _simulationZeroAct (imp spec : BaseModuleWf) (simRel : RegsT -> RegsT ->
                       simRel oImp' oSpec')):
   TraceInclusion (Base imp) (Base spec).
 Proof.
-  eauto using simulationZeroAct.
+  eauto using _simulationZeroAct.
 Qed.
 
-Theorem _simulationGen (imp spec : BaseModuleWf) (NoSelfCalls : NoSelfCallBaseModule spec)
+Theorem simulationGen (imp spec : BaseModuleWf) (NoSelfCalls : NoSelfCallBaseModule spec)
         (simRel : RegsT -> RegsT -> Prop)
         (simRelGood : forall oImp oSpec : RegsT,
             simRel oImp oSpec -> getKindAttr oSpec = getKindAttr (getRegisters spec))
@@ -169,10 +171,10 @@ Theorem _simulationGen (imp spec : BaseModuleWf) (NoSelfCalls : NoSelfCallBaseMo
              exists k, In k (map fst uImpl1) /\ In k (map fst uImpl2)) :
   TraceInclusion (Base imp) (Base spec).
 Proof.
-  eauto using simulationGen.
+  eauto using _simulationGen.
 Qed.
 
-Theorem _simulationGeneralEx (imp spec: BaseModuleWf) (NoSelfCalls: NoSelfCallBaseModule spec)
+Theorem simulationGeneralEx (imp spec: BaseModuleWf) (NoSelfCalls: NoSelfCallBaseModule spec)
         (simRel: RegsT -> RegsT -> Prop)
         (simRelGood: forall oImp oSpec,
             simRel oImp oSpec -> getKindAttr oSpec = getKindAttr (getRegisters spec))
@@ -225,10 +227,10 @@ Theorem _simulationGeneralEx (imp spec: BaseModuleWf) (NoSelfCalls: NoSelfCallBa
              exists k, In k (map fst uImpl1) /\ In k (map fst uImpl2)) :
   TraceInclusion (Base imp) (Base spec).
 Proof.
-  eauto using simulationGeneralEx.
+  eauto using _simulationGeneralEx.
 Qed.
 
-Theorem _simulationZeroA (imp spec: BaseModuleWf) (simRel: RegsT -> RegsT -> Prop)
+Theorem simulationZeroA (imp spec: BaseModuleWf) (simRel: RegsT -> RegsT -> Prop)
         (simRelGood: forall oImp oSpec,
             simRel oImp oSpec ->
             getKindAttr oSpec = getKindAttr (getRegisters spec))
@@ -257,10 +259,10 @@ Theorem _simulationZeroA (imp spec: BaseModuleWf) (simRel: RegsT -> RegsT -> Pro
                         simRel (doUpdRegs uImp oImp) oSpec'))) :
   TraceInclusion (Base imp) (Base spec).
 Proof.
-  eauto using simulationZeroA.
+  eauto using _simulationZeroA.
 Qed.
 
-Theorem _simulationGeneral (imp spec: BaseModuleWf) (NoSelfCalls: NoSelfCallBaseModule spec)
+Theorem simulationGeneral (imp spec: BaseModuleWf) (NoSelfCalls: NoSelfCallBaseModule spec)
         (simRel: RegsT -> RegsT -> Prop)
         (simRelGood: forall oImp oSpec,
             simRel oImp oSpec -> getKindAttr oSpec = getKindAttr (getRegisters spec))
@@ -309,10 +311,10 @@ Theorem _simulationGeneral (imp spec: BaseModuleWf) (NoSelfCalls: NoSelfCallBase
              exists k, In k (map fst uImpl1) /\ In k (map fst uImpl2)) :
   TraceInclusion (Base imp) (Base spec).
 Proof.
-  eauto using simulationGeneral.
+  eauto using _simulationGeneral.
 Qed.
 
-Theorem _simulationZeroAction (imp spec: BaseModuleWf) (simRel: RegsT -> RegsT -> Prop)
+Theorem simulationZeroAction (imp spec: BaseModuleWf) (simRel: RegsT -> RegsT -> Prop)
         (simRelGood: forall oImp oSpec,
             simRel oImp oSpec -> getKindAttr oSpec = getKindAttr (getRegisters spec))
         (simRelImpGood: forall oImp oSpec,
@@ -337,103 +339,80 @@ Theorem _simulationZeroAction (imp spec: BaseModuleWf) (simRel: RegsT -> RegsT -
                       simRel (doUpdRegs uImp oImp) (doUpdRegs uSpec oSpec)))) :
   TraceInclusion (Base imp) (Base spec).
 Proof.
-  eauto using simulationZeroAction.
+  eauto using _simulationZeroAction.
 Qed.
 
-Theorem _WfConcatAssoc1 (m1 m2 m3 : Mod) :
+Theorem WfMod_Concat_assoc_1 (m1 m2 m3 : Mod) :
   WfMod (ConcatMod m1 (ConcatMod m2 m3)) -> WfMod (ConcatMod (ConcatMod m1 m2) m3).
 Proof.
   eauto using WfConcatAssoc1.
 Qed.
 
-Theorem _WfConcatAssoc2 (m1 m2 m3 : Mod) :
+Theorem WfMod_Concat_assoc_2 (m1 m2 m3 : Mod) :
   WfMod (ConcatMod (ConcatMod m1 m2) m3) -> WfMod (ConcatMod m1 (ConcatMod m2 m3)).
 Proof.
   eauto using WfConcatAssoc2.
 Qed.
 
-Theorem _WfModBreakDownFile (m : Mod) :
+Theorem WfMod_BreakDownFile (m : Mod) :
   WfMod m -> WfMod (mergeSeparatedBaseFile (fst (snd (separateMod m)))).
 Proof.
   eauto using WfModBreakDownFile.
 Qed.
 
-Theorem _WfModBreakDownMod (m : Mod) :
+Theorem WfMod_BreakDownMod (m : Mod) :
   WfMod m -> WfMod (mergeSeparatedBaseMod (snd (snd (separateMod m)))).
 Proof.
   eauto using WfModBreakDownMod.
 Qed.
 
-Theorem _merged_WellFormed (m : Mod) :
+Theorem WfMod_merge (m : Mod) :
   WfMod m -> WfMod (mergeSeparatedMod (separateMod m)).
 Proof.
   eauto using merged_WellFormed.
 Qed.
 
-Theorem _WfMod_getFlat (m : Mod) :
+Theorem WfMod_getFlat (m : Mod) :
   WfMod m -> WfMod (getFlat m).
 Proof.
-  eauto using WfMod_getFlat.
+  eauto using _WfMod_getFlat.
 Qed.
 
-Theorem _TraceInclusion_Merge_l (m : ModWf) :
-  TraceInclusion m (WfMergedMod m).
+Definition merge_ModWf m := WfMergedMod m.
+
+Theorem TraceInclusion_merge_r (m : ModWf) :
+  TraceInclusion m (merge_ModWf m).
 Proof.
   eauto using TraceInclusion_Merge_l.
 Qed.
 
-Theorem _TraceInclusion_Merge_r (m : ModWf) :
-  TraceInclusion (WfMergedMod m) m.
+Theorem TraceInclusion_merge_l (m : ModWf) :
+  TraceInclusion (merge_ModWf m) m.
 Proof.
   eauto using TraceInclusion_Merge_r.
 Qed.
 
-Theorem _ConcatMod_comm (m1 m2 : Mod) : 
+Theorem TraceInclusion_ConcatMod_comm (m1 m2 : Mod) : 
   WfMod (ConcatMod m1 m2) -> TraceInclusion (ConcatMod m1 m2) (ConcatMod m2 m1).
 Proof.
   eauto using ConcatMod_comm.
 Qed.
 
-Theorem _ConcatModAssoc1 (m1 m2 m3 : Mod) :
+Theorem TraceInclusion_ConcatMod_assoc_1 (m1 m2 m3 : Mod) :
   WfMod (ConcatMod (ConcatMod m1 m2) m3) ->
   TraceInclusion (ConcatMod m1 (ConcatMod m2 m3)) (ConcatMod (ConcatMod m1 m2) m3).
 Proof.
   eauto using ConcatModAssoc1.
 Qed.
 
-Theorem _ConcatModAssoc2 (m1 m2 m3 : Mod) :
+Theorem TraceInclusion_ConcatMod_assoc_2 (m1 m2 m3 : Mod) :
   WfMod (ConcatMod (ConcatMod m1 m2) m3) ->
   TraceInclusion (ConcatMod (ConcatMod m1 m2) m3) (ConcatMod m1 (ConcatMod m2 m3)).
 Proof.
   eauto using ConcatModAssoc2.
 Qed.
 
-(*
-PPlusProperties.v:Theorem flatten_inline_remove_TraceInclusion (m : ModWf) :
- *)
-
-Theorem _StrongPPlusTraceInclusion_PPlusTraceInclusion (m m' : BaseModule) :
-  StrongPPlusTraceInclusion m m' -> PPlusTraceInclusion m m'.
-Proof.
-  eauto using StrongPPlusTraceInclusion_PPlusTraceInclusion.
-Qed.
-
-Theorem _PPlusTraceInclusion_PTraceInclusion (m m' : BaseModule) :
-  PPlusTraceInclusion m m' -> PTraceInclusion m m'.
-Proof.
-  eauto using PPlusTraceInclusion_PTraceInclusion.
-Qed.
-
-Theorem _PPlusTraceInclusion_TraceInclusion (m m' : BaseModule) :
-  WfMod m ->
-  WfMod m' ->
-  PPlusTraceInclusion m m' ->
-  TraceInclusion m m'.
-Proof.
-  eauto using PPlusTraceInclusion_TraceInclusion.
-Qed.
-
-Theorem _TraceInclusion_inlining_Rules_r (m : BaseModule) (f : DefMethT) (rn : string):
+Theorem TraceInclusion_inlineSingle_Rule_BaseModule_r (m : BaseModule) (f : DefMethT) (rn : string):
   In f (getMethods m) ->
   WfMod m ->
   TraceInclusion m (inlineSingle_Rule_BaseModule f rn m).
@@ -441,7 +420,7 @@ Proof.
   eauto using TraceInclusion_inlining_Rules_r.
 Qed.
 
-Theorem _TraceInclusion_inlining_Meth_r (m : BaseModule) (f : DefMethT) (gn : string) :
+Theorem TraceInclusion_inlineSingle_Meth_BaseModule_r (m : BaseModule) (f : DefMethT) (gn : string) :
   In f (getMethods m) ->
   WfMod m ->
   TraceInclusion m (inlineSingle_Meth_BaseModule f gn m).
@@ -449,7 +428,7 @@ Proof.
   eauto using TraceInclusion_inlining_Meth_r.
 Qed.
 
-Theorem _inline_meth_transform (f : DefMethT) (regs : list RegInitT)
+Theorem TraceInclusion_inline_Meth_transform_r (f : DefMethT) (regs : list RegInitT)
         (rules : list RuleT) (meths : list DefMethT):
   WfMod (BaseMod regs rules meths) ->
   In f meths ->
@@ -460,7 +439,7 @@ Proof.
   eauto using inline_meth_transform.
 Qed.
 
-Theorem _inline_rule_transform (f : DefMethT) (regs : list RegInitT)
+Theorem TraceInclusion_inline_Rule_transform_r (f : DefMethT) (regs : list RegInitT)
         (rules : list RuleT) (meths : list DefMethT):
   WfMod (BaseMod regs rules meths) ->
   In f meths ->
@@ -471,7 +450,7 @@ Proof.
   eauto using inline_rule_transform.
 Qed.
 
-Theorem _inline_meth_fold_right (f : DefMethT) (regs : list RegInitT)
+Theorem TraceInclusion_inline_Meth_fold_right_r (f : DefMethT) (regs : list RegInitT)
         (rules : list RuleT) (meths : list DefMethT):
   WfMod (BaseMod regs rules meths) ->
   forall xs : list nat,
@@ -482,7 +461,7 @@ Proof.
   eauto using inline_meth_fold_right.
 Qed.
 
-Theorem _inline_rule_fold_right (f : DefMethT) (regs : list RegInitT)
+Theorem TraceInclusion_inline_Rule_fold_right_r (f : DefMethT) (regs : list RegInitT)
         (rules : list RuleT) (meths : list DefMethT):
   WfMod (BaseMod regs rules meths) ->
   forall xs : list nat,
@@ -493,7 +472,7 @@ Proof.
   eauto using inline_rule_fold_right.
 Qed.
 
-Theorem _TraceInclusion_inline_BaseModule_rules (regs : list RegInitT) (rules : list RuleT)
+Theorem TraceInclusion_inlineSingle_Rule_r (regs : list RegInitT) (rules : list RuleT)
         (meths : list DefMethT) (f : DefMethT):
   WfMod (BaseMod regs rules meths) ->
   In f meths ->
@@ -503,7 +482,7 @@ Proof.
   eauto using TraceInclusion_inline_BaseModule_rules.
 Qed.
 
-Theorem _TraceInclusion_inline_BaseModule_meths (regs : list RegInitT)
+Theorem TraceInclusion_inlineSingle_Meth_r (regs : list RegInitT)
         (rules : list RuleT) (meths : list DefMethT) (f : DefMethT):
   WfMod (BaseMod regs rules meths) ->
   In f meths ->
@@ -513,7 +492,7 @@ Proof.
   eauto using TraceInclusion_inline_BaseModule_meths.
 Qed.
 
-Theorem _TraceInclusion_inline_BaseModule_all (regs : list RegInitT) (rules : list RuleT)
+Theorem TraceInclusion_inlineSingle_BaseModule_r (regs : list RegInitT) (rules : list RuleT)
         (meths : list DefMethT) (f : DefMethT):
   WfMod (BaseMod regs rules meths) ->
   In f meths ->
@@ -522,7 +501,7 @@ Proof.
   eauto using TraceInclusion_inline_BaseModule_all.
 Qed.
 
-Theorem _TraceInclusion_inlineSingle_pos_Rules (regs : list RegInitT) (rules : list RuleT)
+Theorem TraceInclusion_inlineSingle_Rules_pos_r (regs : list RegInitT) (rules : list RuleT)
         (meths : list DefMethT):
   WfMod (BaseMod regs rules meths) ->
   forall n : nat,
@@ -533,7 +512,7 @@ Proof.
   eauto using TraceInclusion_inlineSingle_pos_Rules.
 Qed.
 
-Theorem _TraceInclusion_inlineAll_pos_Rules (regs : list RegInitT) (rules : list RuleT)
+Theorem TraceInclusion_inlineAll_Rules_BaseMod_r (regs : list RegInitT) (rules : list RuleT)
         (meths : list DefMethT):
   WfMod (BaseMod regs rules meths) ->
   WfMod (BaseMod regs (inlineAll_Rules meths rules) meths) /\
@@ -543,7 +522,7 @@ Proof.
   eauto using TraceInclusion_inlineAll_pos_Rules.
 Qed.
 
-Theorem _TraceInclusion_inlineSingle_pos_Meths (regs : list RegInitT) (rules : list RuleT)
+Theorem TraceInclusion_inlineSingle_Meths_pos_r (regs : list RegInitT) (rules : list RuleT)
         (meths : list DefMethT):
   WfMod (BaseMod regs rules meths) ->
   forall n : nat,
@@ -554,7 +533,7 @@ Proof.
   eauto using TraceInclusion_inlineSingle_pos_Meths.
 Qed.
 
-Theorem _TraceInclusion_inlineAll_pos_Meths (regs : list RegInitT) (rules : list RuleT)
+Theorem TraceInclusion_inlineAll_Meths_BaseMod_r (regs : list RegInitT) (rules : list RuleT)
         (meths : list DefMethT):
   WfMod (BaseMod regs rules meths) ->
   WfMod (BaseMod regs rules (inlineAll_Meths meths)) /\
@@ -563,7 +542,7 @@ Proof.
   eauto using TraceInclusion_inlineAll_pos_Meths.
 Qed.
 
-Theorem _TraceInclusion_inlineAll_pos (regs : list RegInitT) (rules : list RuleT)
+Theorem TraceInclusion_inlineAll_All_r (regs : list RegInitT) (rules : list RuleT)
         (meths : list DefMethT):
   WfMod (BaseMod regs rules meths) ->
   WfMod (inlineAll_All regs rules meths) /\
@@ -572,56 +551,56 @@ Proof.
   eauto using TraceInclusion_inlineAll_pos.
 Qed.
 
-Theorem _WfCreateHide_Mod (m : ModWf) :
+Theorem WfMod_flatten_inline_everything (m : ModWf) :
   WfMod (flatten_inline_everything m).
 Proof.
   eauto using WfCreateHide_Mod.
 Qed.
 
-Theorem _TraceInclusion_flatten_inline_everything_r (m : ModWf) :
+Theorem TraceInclusion_flatten_inline_everything_r (m : ModWf) :
   TraceInclusion m (inlined_ModWf m).
 Proof.
-  eauto using TraceInclusion_flatten_inline_everything_r.
+  eauto using _TraceInclusion_flatten_inline_everything_r.
 Qed.
 
-Theorem _inlineSingle_Rule_map_Wf {f : DefMethT} {m : ModWf} (inMeths : In f (getAllMethods m)):
+Theorem WfMod_inlineSingle_Rule_map {f : DefMethT} {m : ModWf} (inMeths : In f (getAllMethods m)):
   WfMod (createHide (inlineSingle_Rule_map_BaseModule f (getFlat m)) (getHidden m)).
 Proof.
   eauto using inlineSingle_Rule_map_Wf.
 Qed.
 
-Theorem _inlineSingle_Meth_map_Wf {m : ModWf} {f : DefMethT} (inMeths : In f (getAllMethods m)) :
+Theorem WfMod_inlineSingle_Meth_map {f : DefMethT} {m : ModWf} (inMeths : In f (getAllMethods m)) :
   WfMod (createHide (inlineSingle_Meth_map_BaseModule f (getFlat m)) (getHidden m)).
 Proof.
   eauto using inlineSingle_Meth_map_Wf.
 Qed.
 
-Theorem _inlineSingle_Rule_map_TraceInclusion {m : ModWf} {f : DefMethT} (inMeths : In f (getAllMethods m)):
+Theorem TraceInclusion_inlineSingle_Rule_map {m : ModWf} {f : DefMethT} (inMeths : In f (getAllMethods m)):
   TraceInclusion m (inlineSingle_Rule_map_ModWf inMeths).
 Proof.
   eauto using inlineSingle_Rule_map_TraceInclusion.
 Qed.
 
-Theorem _inlineSingle_Meth_map_TraceInclusion {m : ModWf}  {f : DefMethT} (inMeths : In f (getAllMethods m)) :
+Theorem TraceInclusion_inlineSingle_Meth_map {m : ModWf}  {f : DefMethT} (inMeths : In f (getAllMethods m)) :
   TraceInclusion m (inlineSingle_Meth_map_ModWf inMeths).
 Proof.
   eauto using inlineSingle_Meth_map_TraceInclusion.
 Qed.
 
-Theorem _inlineSingle_Module_Wf {m : ModWf} {f : DefMethT} (inMeths : In f (getAllMethods m)) :
+Theorem WfMod_inlineSingle_Module {m : ModWf} {f : DefMethT} (inMeths : In f (getAllMethods m)) :
   WfMod (inlineSingle_Module f m).
 Proof.
   eauto using inlineSingle_Module_Wf.
 Qed.
 
-Theorem _inlineSingle_BaseModule_TraceInclusion {m : ModWf} {f : DefMethT}
+Theorem TraceInclusion_inlineSingle_Module_ModWf_r {m : ModWf} {f : DefMethT}
         (inMeths : In f (getAllMethods m)) :
   TraceInclusion m (inlineSingle_Module_ModWf inMeths).
 Proof.
   eauto using inlineSingle_BaseModule_TraceInclusion.
 Qed.
 
-Theorem _inlineSingle_BaseModule_nth_Meth_Wf {m : ModWf} {f : DefMethT}
+Theorem WfMod_inlineSingle_BaseModule_nth_Meth {m : ModWf} {f : DefMethT}
         (inMeths : In f (getAllMethods m)) (xs : list nat) :
   WfMod
     (createHide
@@ -631,14 +610,14 @@ Proof.
   eauto using inlineSingle_BaseModule_nth_Meth_Wf.
 Qed.
 
-Theorem _inlineSingle_BaseModule_nth_Meth_TraceInclusion {m : ModWf} {f : DefMethT}
+Theorem TraceInclusion_inlineSingle_BaseModule_nth_Meth_r {m : ModWf} {f : DefMethT}
         (inMeths : In f (getAllMethods m)) (xs : list nat) :
   TraceInclusion m (inlineSingle_BaseModule_nth_Meth_ModWf inMeths xs).
 Proof.
   eauto using inlineSingle_BaseModule_nth_Meth_TraceInclusion.
 Qed.
 
-Theorem _inlineSingle_BaseModule_nth_Rule_Wf {m : ModWf} {f : DefMethT}
+Theorem WfMod_inlineSingle_BaseModule_nth_Rule {m : ModWf} {f : DefMethT}
         (inMeths : In f (getAllMethods m)) (xs : list nat) :
   WfMod
     (createHide
@@ -648,59 +627,59 @@ Proof.
   eauto using inlineSingle_BaseModule_nth_Rule_Wf.
 Qed.
 
-Theorem _inlineSingle_BaseModule_nth_Rule_TraceInclusion {m : ModWf} {f : DefMethT} (inMeths : In f (getAllMethods m)) (xs : list nat) :
+Theorem TraceInclusion_inlineSingle_BaseModule_nth_Rule_r {m : ModWf} {f : DefMethT} (inMeths : In f (getAllMethods m)) (xs : list nat) :
   TraceInclusion m (inlineSingle_BaseModule_nth_Rule_ModWf inMeths xs).
 Proof.
   eauto using inlineSingle_BaseModule_nth_Rule_TraceInclusion.
 Qed.
 
-Theorem _inlineAll_Rules_Wf (m : ModWf):
+Theorem WfMod_inlineAll_Rules (m : ModWf):
   WfMod (inlineAll_Rules_Mod m).
 Proof.
   eauto using inlineAll_Rules_Wf.
 Qed.
 
-Theorem _inlineAll_Rules_TraceInclusion (m : ModWf) :
+Theorem TraceInclusion_inlineAll_Rules_r (m : ModWf) :
   TraceInclusion m (inlineAll_Rules_ModWf m).
 Proof.
   eauto using inlineAll_Rules_TraceInclusion.
 Qed.
 
-Theorem _inlineAll_Meths_Wf (m : ModWf) :
+Theorem WfMod_inlineAll_Meths (m : ModWf) :
   WfMod (inlineAll_Meths_Mod m).
 Proof.
   eauto using inlineAll_Meths_Wf.
 Qed.
 
-Theorem _inlineAll_Meths_TraceInclusion (m : ModWf) :
+Theorem TraceInclusion_inlineAll_Meths_r (m : ModWf) :
   TraceInclusion m (inlineAll_Meths_ModWf m).
 Proof.
   eauto using inlineAll_Meths_TraceInclusion.
 Qed.
 
-Theorem _flatten_inline_remove_Wf (m : ModWf) :
+Theorem WfMod_flatten_inline_remove (m : ModWf) :
   WfMod (flatten_inline_remove m).
 Proof.
   eauto using flatten_inline_remove_Wf.
 Qed.
 
-Theorem _removeHides_createHide_TraceInclusion (m : BaseModuleWf) (l : list string)
+Theorem TraceInclusion_removeHides_createHide (m : BaseModuleWf) (l : list string)
         (subList : SubList l (map fst (getMethods m))):
   NoSelfCallBaseModule m ->
-  TraceInclusion (removeHidesModWf m l) (createHideModWf m subList).
+  TraceInclusion (removeHides_ModWf m l) (createHide_ModWf m subList).
 Proof.
   eauto using removeHides_createHide_TraceInclusion.
 Qed.
 
-Theorem _createHide_removeHides_TraceInclusion (m : BaseModuleWf) (l : list string)
+Theorem TraceInclusion_createHide_removeHides (m : BaseModuleWf) (l : list string)
         (subList : SubList l (map fst (getMethods m))):
   NoSelfCallBaseModule m ->
-  TraceInclusion (createHideModWf m subList) (removeHidesModWf m l).
+  TraceInclusion (createHide_ModWf m subList) (removeHides_ModWf m l).
 Proof.
   eauto using createHide_removeHides_TraceInclusion.
 Qed.
 
-Theorem _flatten_inline_remove_TraceInclusion (m : ModWf) :
+Theorem TraceInclusion_flatten_inline_everything_flatten_inline_remove (m : ModWf) :
   NoSelfCallBaseModule (inlineAll_All_mod m) ->
   TraceInclusion (flatten_inline_everything m) (flatten_inline_remove_ModWf m).
 Proof.
